\begin{problem}
  Prove integration by parts.
  That is, suppose $F$ and $G$ are continuously differentiable functions on $[a, b]$.
  Then, prove that
  \[
    \int\limits_a^b F(x)G'(x) \d x = F(b)G(b) - F(a)G(a) - \int\limits_a^b F'(x)G(x) \d x.
  \]
\end{problem}

% \begin{answer}
  \begin{proof}
    Since $F$ and $G$ are continuously differentiable on $[a, b]$,
    they are also continuous on $[a, b]$.
    Thus, by the fundamental theorem of calculus, we have
    Let $H(x) = F(x)G(x)$, then
    \begin{align*}
      H'(x) &= \frac{d}{dx} \brackets{F(x)G(x)} \\
            &= F'(x)G(x) + F(x)G'(x) \qquad \blue{\text{(by the product rule)}}. \\
      \intertext{ What happens if we integrate both sides of this equation? }
      \int\limits_a^b H'(x) \d x &= \int\limits_a^b \brackets{F'(x)G(x) + F(x)G'(x)} \d x \\
      H(b) - H(a) &= \int\limits_a^b F'(x)G(x) \d x + \int\limits_a^b F(x)G'(x) \d x
    \end{align*}
    Rearranging this gives us
    \[
      H(b) - H(a) - \int\limits_a^b F'(x)G(x) \d x = \int\limits_a^b F(x)G'(x) \d x
    \]

    Since $H(x) = F(x)G(x)$, we have
    \blue{\[
      \int\limits_a^b F(x)G'(x) \d x = F(b)G(b) - F(a)G(a) - \int\limits_a^b F'(x)G(x) \d x
    \]}
  \end{proof}
% \end{answer}
